* http://sicp.iijlab.net/fulltext/x122.html#ex113

```
φ = (1 + √5) / 2
ψ = (1 - √5) / 2
```
とした場合、`Fib(n) = f(n) = (φ^n - ψ^n) / √5` であることを証明するため、
n = 0, n = 1, n > 1 の場合で、確かめてみる

## n = 0
```
Fib(0) = 0

f(0)
= (((1-√5)/2)^0 - ((1-√5)/2)^0) / √5
= (1 - 1) / √5
= 0
```

## n = 1

```
Fib(1) = 1

f(1)
= (((1-√5)/2)^1 - ((1-√5)/2)^1) / √5
= ((1-√5) / 2 - (1-√5) / 2) / √5
= √5 / √5
= 1
```

## n > 1

```
Fib(n) = Fib(n-1) + Fib(n-2)

f(n)
= (φ^n - ψ^n) / √5
= ((φ^(n-2) * φ^2) - (ψ^(n-2) * ψ^2)) / √5
= ((φ^(n-2) * (φ + 1)) - (ψ^(n-2) * (ψ + 1))) / √5      ;; この部分への展開は、下記を参照
= ((φ^(n-1) + φ^(n-2)) - (ψ^(n-1) + ψ^(n-2))) / √5
= (φ^(n-1) - ψ^(n-1)) / √5 + (φ^(n-2) - ψ^(n-2)) / √5
= Fib(n-1) + Fib(n-2)

φ^2
= ((1 + √5) / 2) ^ 2
= (1 + 2√5 + 5) / 4
= (2 + 2√5 + 4) / 4
= (1 + √5 / 2) + 1
= φ + 1

ψ^2
= ((1 - √5) / 2) ^ 2
= (1 - 2√5 + 5) / 4
= (2 - 2√5 + 4) / 4
= (1 - √5 / 2) + 1
= ψ + 1
```
